proof-libs/fstar/core/Core.Result.fst
@@ -1,7 +1,6 @@
 module Core.Result
 
-type t_Result t e = | Result_Ok: v:t -> t_Result t e
-                    | Result_Err of e
+include Core.Result_Option_bundle {t_Result, impl__ok}
 
 let impl__unwrap #t #e (x: t_Result t e {Result_Ok? x}): t = Result_Ok?.v x
 let impl__map_err #e1 #e2 (x: t_Result 't e1) (f: e1 -> e2): t_Result 't e2
@@ -23,4 +22,5 @@ let impl__and_then #t #e #u (self: t_Result t e) (op: t -> t_Result u e): t_Resu
   match self with 
   | Result_Ok v -> op v 
   | Result_Err e -> Result_Err e
+
 
