proof-libs/fstar/core/Core.Result_Option_bundle.fst
@@ -1,0 +1,21 @@
+module Core.Result_Option_bundle
+
+type t_Result t e = | Result_Ok: v:t -> t_Result t e
+                    | Result_Err of e
+
+type t_Option t = | Option_Some of t | Option_None
+
+let impl__ok #t #e (self: t_Result t e): t_Option t = 
+  match self with 
+  | Result_Ok v -> Option_Some v
+  | Result_Err _ -> Option_None 
+
+let impl__ok_or_else #t_Self #e (self: t_Option t_Self) (err: unit -> e): t_Result t_Self e =
+  match self with 
+  | Option_Some inner -> Result_Ok inner
+  | Option_None -> Result_Err (err ())
+
+let impl__ok_or #t_Self #e (self: t_Option t_Self) (err: e): t_Result t_Self e =
+  match self with 
+  | Option_Some inner -> Result_Ok inner
+  | Option_None -> Result_Err err
