proof-libs/fstar/core/Core.Slice.fsti
@@ -37,3 +37,18 @@ val impl__split_at #t (s: t_Slice t) (mid: usize): Pure (t_Slice t * t_Slice t)
 
 let impl__is_empty (s: t_Slice 'a): bool = Seq.length s = 0
 
+val impl__copy_within
+      (#v_T #v_R: Type0)
+      (* (#[FStar.Tactics.Typeclasses.tcresolve
+            ()]
+          i2:
+          Core.Ops.Range.t_RangeBounds v_R
+            usize) *)
+      (#[FStar.Tactics.Typeclasses.tcresolve
+            ()]
+          i3:
+          Core.Marker.t_Copy v_T)
+      (v: t_Slice v_T)
+      (src: v_R)
+      (dest: usize)
+    : t_Slice v_T
